theories/MaxOfTwoNumbersUndertrainedSimpler/Computed/AllPostembed.v
@@ -8,11 +8,12 @@ Set NativeCompute Timing.
 Time #[native_compile=no] Local Definition centered_residual_error_m1_concrete_value := native_compute centered_residual_error_m1_concrete_opt.
 
 Time #[native_compile=no] Definition centered_residual_error_m1_concrete : PArray.concrete_tensor _ _ := (*Eval native_compute in pre *)Eval hnf in extract centered_residual_error_m1_concrete_value.
-Time Definition centered_residual_error_m1_concrete_eq : centered_residual_error_m1_concrete = centered_residual_error_m1_concrete_opt := extract_eq centered_residual_error_m1_concrete_value. (*
+(* Drop #[native_compile=no] in all definitions after this line once the attribute is automatically transitively recursive, cf https://github.com/coq/coq/pull/18033#issuecomment-1746899653 *)
+Time #[native_compile=no] Definition centered_residual_error_m1_concrete_eq : centered_residual_error_m1_concrete = centered_residual_error_m1_concrete_opt := extract_eq centered_residual_error_m1_concrete_value. (*
 Proof. native_cast_no_check (eq_refl residual_error_m1_all_tokens_concrete). Time Qed.*)
 
-Definition centered_residual_error_m1 : tensor _ _ := PArray.reabstract (fun _ => centered_residual_error_m1_float) centered_residual_error_m1_concrete.
-Lemma centered_residual_error_m1_eq idxs : centered_residual_error_m1 idxs = centered_residual_error_m1_float idxs.
+#[native_compile=no] Definition centered_residual_error_m1 : tensor _ _ := PArray.reabstract (fun _ => centered_residual_error_m1_float) centered_residual_error_m1_concrete.
+#[native_compile=no] Lemma centered_residual_error_m1_eq idxs : centered_residual_error_m1 idxs = centered_residual_error_m1_float idxs.
 Proof.
   cbv [centered_residual_error_m1].
   rewrite PArray.reabstract_ext_correct; [ reflexivity | ].
