theories/MaxOfTwoNumbers/Theorems/Attempt_01_BruteForce.v
@@ -8,7 +8,8 @@ From NeuralNetInterp.MaxOfTwoNumbers.Computed Require Import AllLogits.
 Local Open Scope uint63_scope.
 Local Open Scope core_scope.
 
-Derive computed_accuracy SuchThat (computed_accuracy = real_accuracy) As computed_accuracy_eq.
+(* Drop #[native_compile=no] in all definitions after this line once the attribute is automatically transitively recursive, cf https://github.com/coq/coq/pull/18033#issuecomment-1746899653 *)
+#[native_compile=no] Derive computed_accuracy SuchThat (computed_accuracy = real_accuracy) As computed_accuracy_eq.
 Proof.
   cbv [real_accuracy].
   etransitivity; revgoals.
