theories/MaxOfTwoNumbersSimpler/Computed/logit_delta.v
@@ -4,9 +4,10 @@ From NeuralNetInterp.Torch Require Import Tensor.Instances.
 From NeuralNetInterp.MaxOfTwoNumbersSimpler Require Import Model Model.ExtraComputations.
 From NeuralNetInterp.MaxOfTwoNumbersSimpler.Computed Require Import AllLogits.
 
-Time #[local] Definition pre_logit_delta := logit_delta_float_gen (all_tokens (use_checkpoint:=false)) all_tokens_logits.
-Time #[local] Definition logit_delta_value := vm_compute pre_logit_delta.
+(* Drop #[native_compile=no] in all definitions after this line once the attribute is automatically transitively recursive, cf https://github.com/coq/coq/pull/18033#issuecomment-1746899653 *)
+Time #[local,native_compile=no] Definition pre_logit_delta := logit_delta_float_gen (all_tokens (use_checkpoint:=false)) all_tokens_logits.
+Time #[local,native_compile=no] Definition logit_delta_value := vm_compute pre_logit_delta.
 
 Time Definition logit_delta := (*Eval native_compute in pre *)Eval hnf in extract logit_delta_value.
 #[local] Strategy -100 [pre_logit_delta].
-Time Definition logit_delta_eq : logit_delta = ltac:(let v := eval cbv delta [pre_logit_delta] in pre_logit_delta in exact v) := extract_eq logit_delta_value.
+Time #[native_compile=no] Definition logit_delta_eq : logit_delta = ltac:(let v := eval cbv delta [pre_logit_delta] in pre_logit_delta in exact v) := extract_eq logit_delta_value.
